Weidenbach_Book/IsaSAT_Literals_LLVM.thy
@@ -1,7 +1,6 @@
 theory IsaSAT_Literals_LLVM
   imports WB_More_Word IsaSAT_Literals Watched_Literals.WB_More_IICF_LLVM
 begin
-
 (* TODO: Move
   TODO:  Write generic postprocessing for that!
   Maybe just beta contraction of form (\<lambda>x. f x)$x = f$x
